tuned

brainfuck_core.thy
@@ -67,4 +67,24 @@ fun eval_basic :: "bf_cmd_basic list \<Rightarrow> state \<Rightarrow> state" wh
 value "print_state (eval_basic [D, R, P, D, R, P, P, D, R, P, P, P, D, L, L, L] (Normal (Tape [] 0 []) (Inp []) (Outp [])))"
 
 
+inductive eval :: "bf_cmd list \<Rightarrow> nat \<Rightarrow> state \<Rightarrow> state \<Rightarrow> bool" for cmd where
+  "s = s' \<Longrightarrow> pc = 0 \<Longrightarrow> eval cmd pc s s'" |
+  "cmd ! pc =  Basic cb \<Longrightarrow> eval cmd pc s s' \<Longrightarrow> (eval_basic cb s') = s'' \<Longrightarrow> eval cmd pc s s''" 
+  (*TODO control flow*)
+
+
+lemma "eval [] 0 (Normal (Tape [] 0 []) inp outp) (Normal (Tape [] 0 []) inp outp)"
+  by(simp add: eval.intros)
+
+lemma "eval [Basic [P, D]] 0 (Normal (Tape [] 0 []) inp (Outp [])) (Normal (Tape [] 1 []) inp (Outp [1]))"
+  (*apply(auto intro: eval.intros)*)
+     apply(rule eval.intros(2))
+    apply(simp)
+     apply(rule eval.intros(1))
+    apply(simp)
+   apply(simp)
+  apply(simp)
+  done
+
+
 end
